src/Language/PlutusIR/Semantics/Dynamic/Substitution.v
@@ -11,132 +11,117 @@ Local Open Scope string_scope.
 (** * Substitution of terms *)
 
 (** ** Utilities *)
-Definition term_var_bound_by_constructor (c : NamedTerm.constructor) : string :=
+Definition bound_var_in_constructor (c : NamedTerm.constructor) : string :=
   match c with
   | Constructor (VarDecl x _) _ => x
   end.
 
-Definition term_vars_bound_by_binding (b : NamedTerm.Binding) : list string :=
+Definition bound_var_in_binding (b : NamedTerm.Binding) : list string :=
   match b with
   | TermBind _ (VarDecl x _) _ => cons x nil
   | TypeBind (TyVarDecl X _) _ => nil
-  | DatatypeBind (Datatype (TyVarDecl X _) YKs matchFunc cs) => matchFunc :: (rev (map term_var_bound_by_constructor cs))
+  | DatatypeBind (Datatype (TyVarDecl X _) YKs matchFunc cs) => matchFunc :: (rev (map bound_var_in_constructor cs))
   end.
 
-Definition term_vars_bound_by_bindings (bs : list NamedTerm.Binding) : list string := List.concat (map term_vars_bound_by_binding bs).
+Definition bound_vars_in_bindings (bs : list NamedTerm.Binding) : list string := List.concat (map bound_var_in_binding bs).
 
 (** ** Implementation of substitution on terms as inductive datatype *)
-Inductive substitute : name -> Term -> Term -> Term -> Prop :=
-  | S_Let1 : forall x s bs t0 bs',
-      In x (term_vars_bound_by_bindings bs) ->
-      substitute_bindings_nonrec x s bs bs' ->
-      substitute x s (Let NonRec bs t0) (Let NonRec bs' t0)
-  | S_Let2 : forall x s bs t0 bs' t0',
-      ~(In x (term_vars_bound_by_bindings bs)) ->
-      substitute_bindings_nonrec x s bs bs' ->
-      substitute x s t0 t0' ->
-      substitute x s (Let NonRec bs t0) (Let NonRec bs' t0')
-  | S_LetRec1 : forall x s bs t0,
-      In x (term_vars_bound_by_bindings bs)->
+Inductive substitute (x : name) (s : Term) :Term -> Term -> Prop :=
+  | S_LetNonRec_Nil1 : forall t t', 
+      substitute x s t t' ->
+      substitute x s (Let NonRec nil t) (Let NonRec nil t')
+  | S_LetNonRec_Cons1 : forall b b' bs t,
+      In x (bound_var_in_binding b) ->
+      substitute_binding x s b b' ->
+      substitute x s (Let NonRec (b :: bs) t) (Let NonRec (b' :: bs) t)
+  | S_LetNonRec_Cons2 : forall b b' bs bs' t t',
+      ~(In x (bound_var_in_binding b)) ->
+      substitute_binding x s b b' ->
+      substitute x s (Let NonRec bs t) (Let NonRec bs' t') ->
+      substitute x s (Let NonRec (b :: bs) t) (Let NonRec (b' :: bs') t')
+  | S_LetRec1 : forall bs t0,
+      In x (bound_vars_in_bindings bs)->
       substitute x s (Let Rec bs t0) (Let Rec bs t0)
-  | S_LetRec2 : forall x s bs t0 bs' t0',
-      ~(In x (term_vars_bound_by_bindings bs)) ->
-      substitute_bindings_rec x s bs bs' ->
-      substitute x s t0 t0' ->
+  | S_LetRec2 : forall bs t0 bs' t0',
+      ~(In x (bound_vars_in_bindings bs)) ->
+      substitute_letrec x s (Let Rec bs t0) (Let Rec bs' t0') ->
       substitute x s (Let Rec bs t0) (Let Rec bs' t0')
-  | S_Var1 : forall x s,
+  | S_Var1 :
       substitute x s (Var x) s
-  | S_Var2 : forall x s y,
+  | S_Var2 : forall y,
       x <> y ->
       substitute x s (Var y) (Var y)
-  | S_TyAbs : forall x s bX K t0 t0',
+  | S_TyAbs : forall bX K t0 t0',
       substitute x s t0 t0' ->
       substitute x s (TyAbs bX K t0) (TyAbs bX K t0')
-  | S_LamAbs1 : forall x s T t0,
+  | S_LamAbs1 : forall T t0,
       substitute x s (LamAbs x T t0) (LamAbs x T t0)
-  | S_LamAbs2 : forall x s bx T t0 t0',
+  | S_LamAbs2 : forall bx T t0 t0',
       x <> bx ->
       substitute x s t0 t0' ->
       substitute x s (LamAbs bx T t0) (LamAbs bx T t0') 
-  | S_Apply : forall x s t1 t2 t1' t2',
+  | S_Apply : forall t1 t2 t1' t2',
       substitute x s t1 t1' ->
       substitute x s t2 t2' ->
       substitute x s (Apply t1 t2) (Apply t1' t2')
-  | S_Constant : forall x s u,
+  | S_Constant : forall u,
       substitute x s (Constant u) (Constant u)
-  | S_Builtin : forall x s d,
+  | S_Builtin : forall d,
       substitute x s (Builtin d) (Builtin d)
-  | S_TyInst : forall x s t0 T t0',
+  | S_TyInst : forall t0 T t0',
       substitute x s t0 t0' ->
       substitute x s (TyInst t0 T) (TyInst t0' T)
-  | S_Error : forall x s T,
+  | S_Error : forall T,
       substitute x s (Error T) (Error T)
-  | S_IWrap : forall x s F T t0 t0',
+  | S_IWrap : forall F T t0 t0',
       substitute x s t0 t0' ->
       substitute x s (IWrap F T t0) (IWrap F T t0')
-  | S_Unwrap : forall x s t0 t0',
+  | S_Unwrap : forall t0 t0',
       substitute x s t0 t0' ->
       substitute x s (Unwrap t0) (Unwrap t0') 
-      
-with substitute_bindings_nonrec : name -> Term -> list Binding -> list Binding -> Prop :=
-  | S_NilB_NonRec : forall x s, 
-      substitute_bindings_nonrec x s nil nil
-  | S_ConsB_NonRec1 : forall x s b b' bs,
-      In x (term_vars_bound_by_binding b) ->
-      substitute_binding x s b b' ->
-      substitute_bindings_nonrec x s (b :: bs) (b' :: bs)
-  | S_ConsB_NonRec2 : forall x s b b' bs bs',
-      ~(In x (term_vars_bound_by_binding b)) ->
-      substitute_binding x s b b' ->
-      substitute_bindings_nonrec x s bs bs' ->
-      substitute_bindings_nonrec x s (b :: bs) (b' :: bs')
 
-with substitute_bindings_rec : name -> Term -> list Binding -> list Binding -> Prop :=
-  | S_NilB_Rec : forall x s,
-      substitute_bindings_rec x s nil nil
-  | S_ConsB_Rec : forall x s b b' bs bs',
+with substitute_letrec (x : name) (s : Term) : Term -> Term -> Prop :=
+  | S_NilB_Rec : forall t t',
+      substitute x s t t' ->
+      substitute_letrec x s (Let Rec nil t) (Let Rec nil t')
+  | S_ConsB_Rec : forall b b' bs bs' t t',
       substitute_binding x s b b' ->
-      substitute_bindings_rec x s bs bs' ->
-      substitute_bindings_rec x s (b :: bs) (b' :: bs')
+      substitute_letrec x s (Let Rec bs t) (Let Rec bs' t') ->
+      substitute_letrec x s (Let Rec (b :: bs) t) (Let Rec (b' :: bs') t')
 
-with substitute_binding : name -> Term -> Binding -> Binding -> Prop :=
-  | S_TermBind : forall x s strictness bx T t t',
+with substitute_binding (x : name) (s : Term) : Binding -> Binding -> Prop :=
+  | S_TermBind : forall strictness bx T t t',
       substitute x s t t' ->
       substitute_binding x s (TermBind strictness (VarDecl bx T) t) (TermBind strictness (VarDecl bx T) t')
-  | S_TypeBind : forall x s tvd T,
+  | S_TypeBind : forall tvd T,
       substitute_binding x s (TypeBind tvd T) (TypeBind tvd T)
-  | S_DatatypeBind : forall x s dtd,
+  | S_DatatypeBind : forall dtd,
       substitute_binding x s (DatatypeBind dtd) (DatatypeBind dtd).
 
 #[export] Hint Constructors substitute : core.
-#[export] Hint Constructors substitute_bindings_nonrec : core.
-#[export] Hint Constructors substitute_bindings_rec : core.
+#[export] Hint Constructors substitute_letrec : core.
 #[export] Hint Constructors substitute_binding : core.
 
 Scheme substitute__ind := Minimality for substitute Sort Prop
-  with substitute_bindings_nonrec__ind := Minimality for substitute_bindings_nonrec Sort Prop
-  with substitute_bindings_rec__ind := Minimality for substitute_bindings_rec Sort Prop
+  with substitute_letrec__ind := Minimality for substitute_letrec Sort Prop
   with substitute_binding__ind := Minimality for substitute_binding Sort Prop.
 
 Combined Scheme substitute__mutind from 
   substitute__ind, 
-  substitute_bindings_nonrec__ind, 
-  substitute_bindings_rec__ind, 
+  substitute_letrec__ind, 
   substitute_binding__ind.
-
-
 
 (** * Multi-substitutions of types in type annotations *)
 
 Definition env := list (name * Term).
 
-Inductive msubst : env -> Term -> Term -> Prop :=
-  | msubst_nil : forall t,
-      msubst nil t t
-  | msubst_cons : forall x s ss t t' t'',
+Inductive msubst_term : env -> Term -> Term -> Prop :=
+  | msubst_term__nil : forall t,
+      msubst_term nil t t
+  | msubst_term__cons : forall x s ss t t' t'',
       substitute x s t t' ->
-      msubst ss t' t'' ->
-      msubst ((x, s) :: ss) t t''
+      msubst_term ss t' t'' ->
+      msubst_term ((x, s) :: ss) t t''
   .
 
 Inductive msubst_binding : env -> Binding -> Binding -> Prop :=
