src/Language/PlutusIR/Semantics/SemanticEquivalence/CompatibilityLemmas/LetNonRec.v
@@ -7,6 +7,186 @@ Require Import PlutusCert.Language.PlutusIR.Semantics.SemanticEquivalence.Monoto
 
 Require Import Arith.
 
+Lemma In__mdrop : forall {X} ns ss x s,
+    List.In x ns ->
+    @mdrop X ns ((x, s) :: ss) = @mdrop X ns ss.
+Proof.
+  induction ns; intros.
+  - destruct H.
+  - simpl.
+    destruct (x =? a) eqn:Heqb.
+    + apply eqb_eq in Heqb as Heq.
+      subst.
+      reflexivity.
+    + apply eqb_neq in Heqb as Hneq.
+      destruct H.
+      * symmetry in H. 
+        apply Hneq in H.
+        destruct H.
+      * eapply IHns.
+        assumption. 
+Qed.
+
+
+Lemma not_In__mdrop : forall {X} ns ss x s,
+    ~ List.In x ns ->
+    @mdrop X ns ((x, s) :: ss) = (x, s) :: @mdrop X ns ss.
+Proof.
+  induction ns; intros.
+  - reflexivity.
+  - simpl.
+    destruct (x =? a) eqn:Heqb.
+    + apply eqb_eq in Heqb as Heq.
+      subst.
+      exfalso.
+      apply H.
+      left.
+      reflexivity.
+    + apply eqb_neq in Heqb as Hneq.
+      eapply IHns.
+      intros Hcon.
+      apply H.
+      right.
+      assumption.
+Qed.
+
+(*
+Lemma subst_bs_nr__bound_vars : forall x s bs bs',
+    substitute_bindings_nonrec x s bs bs' ->
+    term_vars_bound_by_bindings bs = term_vars_bound_by_bindings bs'.
+Proof.
+  intros.
+  induction H.
+  - reflexivity.
+  - destruct b. 
+    all: inversion H0; subst.
+    all: auto.
+  - destruct b.
+    all: inversion H0. subst.
+    all: unfold term_vars_bound_by_bindings.
+    all: simpl.
+    all: f_equal.
+    all: auto.
+Qed.*)
+
+Lemma substA_bs_nr__bound_tyvars : forall x s bs bs',
+    substituteA_bindings_nonrec x s bs bs' ->
+    tyvars_bound_by_bindings bs = tyvars_bound_by_bindings bs'.
+Proof.
+  intros.
+  induction H.
+  - reflexivity.
+  - destruct b. 
+    all: inversion H0; subst.
+    all: auto.
+  - destruct b.
+    all: inversion H0. subst.
+    all: unfold tyvars_bound_by_bindings.
+    all: simpl.
+    all: try solve [f_equal; auto].
+    apply IHsubstituteA_bindings_nonrec.
+Qed.
+    
+(*
+Lemma msubst_LetNonRec : forall ss bs e t',
+    msubst_term ss (Let NonRec bs e) t' ->
+    exists bs' e', 
+      ForallP (fun b => exists b, msubst )
+      msubst_bindings_nonrec ss bs bs' /\ 
+      msubst_term (mdrop (term_vars_bound_by_bindings bs) ss) e e' /\ 
+      t' = Let NonRec bs' e'.
+Proof.
+  induction ss; intros.
+  - inversion H. subst.
+    exists bs, e.
+    rewrite mdrop_nil.
+    eauto using msubst_bindings_nonrec__nil, msubst_nil, msubst_cons. 
+  - inversion H. subst.
+    rename t'0 into e''.
+    inversion H2.
+    + subst.
+      apply IHss in H5.
+      destruct H5 as [bs'' [e'' [H9 [H10 H11]]]].
+      subst.
+      exists bs'', e''.
+      split. {
+        apply msubst_bindings_nonrec__cons with bs'.
+        + assumption.
+        + apply H9.
+      }
+      split. {
+        rewrite In__mdrop; auto.
+        erewrite subst_bs_nr__bound_vars; eauto.
+      }
+      reflexivity.
+    + subst.
+      rename t0' into e'.
+      apply IHss in H5.
+      destruct H5 as [bs'' [e'' [H10 [H11 H12]]]].
+      subst.
+      exists bs'', e''.
+      split. {
+        apply msubst_bindings_nonrec__cons with bs'.
+        + assumption.
+        + apply H10.
+      }
+      split. {
+        rewrite not_In__mdrop; auto.
+        eapply msubst_cons; eauto. 
+        erewrite subst_bs_nr__bound_vars; eauto.
+      }
+      reflexivity.
+Qed.
+
+Lemma msubstA_LetNonRec : forall ss bs e t',
+    msubstA ss (Let NonRec bs e) t' ->
+    exists bs' e', 
+      msubstA_bindings_nonrec ss bs bs' /\ 
+      msubstA (mdrop (tyvars_bound_by_bindings bs) ss) e e' /\ 
+      t' = Let NonRec bs' e'.
+Proof.
+  induction ss; intros.
+  - inversion H. subst.
+    exists bs, e.
+    rewrite mdrop_nil.
+    eauto using msubstA_bindings_nonrec__nil, msubstA_nil, msubstA_cons. 
+  - inversion H. subst.
+    rename t'0 into e''.
+    inversion H2.
+    + subst.
+      apply IHss in H5.
+      destruct H5 as [bs'' [e'' [H9 [H10 H11]]]].
+      subst.
+      exists bs'', e''.
+      split. {
+        apply msubstA_bindings_nonrec__cons with bs'.
+        + assumption.
+        + apply H9.
+      }
+      split. {
+        rewrite In__mdrop; auto.
+        erewrite substA_bs_nr__bound_tyvars; eauto.
+      }
+      reflexivity.
+    + subst.
+      rename t0' into e'.
+      apply IHss in H5.
+      destruct H5 as [bs'' [e'' [H10 [H11 H12]]]].
+      subst.
+      exists bs'', e''.
+      split. {
+        apply msubstA_bindings_nonrec__cons with bs'.
+        + assumption.
+        + apply H10.
+      }
+      split. {
+        rewrite not_In__mdrop; auto.
+        eapply msubstA_cons; eauto. 
+        erewrite substA_bs_nr__bound_tyvars; eauto.
+      }
+      reflexivity.
+Qed. *)
+
 Lemma compatibility_LetNonRec : forall Delta Gamma bs t bs' t' T,
     forall Delta' Gamma',
       (Delta', Gamma') = append (flatten (List.map binds bs)) (Delta, Gamma) ->
@@ -18,7 +198,7 @@ Proof.
   unfold LR_logically_approximate.
 
   split. {
-    eapply T_Let.
+    eapply T_Let. 
     - apply Hbinds.
     - eapply LR_la_bnr__oks in IH_LR__bs. 
       apply IH_LR__bs. 
@@ -39,15 +219,15 @@ Proof.
   intros k rho env env' ct ck HeqDelta HeqGamma [H_RD H_RG].
   subst.
 
-  (*
-  intros e_sa e'_sa e_s e'_s.
-  intros HmsA__e_sa HmsA__e'_sa Hms__e_s Hms__e'_s.
+  intros e_msa e'_msa e_ms e'_ms.
+  intros HmsA__e_msa HmsA__e'_msa Hms__e_ms Hms__e'_ms.
 
-  destruct (msubstA_LamAbs _ _ _ _ _ HmsA__e_sa) as [eb_sa [HmsA__eb_sa Heq]].
-  destruct (msubstA_LamAbs _ _ _ _ _ HmsA__e'_sa) as [eb'_sa [HmsA__eb'_sa Heq']].
+  (*
+  destruct (msubstA_LetNonRec _ _ _ _ HmsA__e_msa) as [bs_msa [t_msa [HmsA__bs_msa [HmsA__t_msa Heq]]]].
+  destruct (msubstA_LetNonRec _ _ _ _ HmsA__e'_msa) as [bs'_msa [t'_msa [HmsA__bs'_msa [HmsA__t'_msa Heq']]]].
   subst.
-  destruct (msubst_LamAbs _ _ _ _ _ Hms__e_s) as [eb_s [Hms__eb_s Heq]].
-  destruct (msubst_LamAbs _ _ _ _ _ Hms__e'_s) as [eb'_s [Hms__eb'_s Heq']].
+  destruct (msubst_LetNonRec _ _ _ _ Hms__e_ms) as [bs_ms [t_ms [Hms__bs_ms [Hms__t_ms Heq]]]].
+  destruct (msubst_LetNonRec _ _ _ _ Hms__e'_ms) as [bs'_ms [t'_ms [Hms__bs'_ms [Hms__t'_ms Heq']]]].
   subst.
 
   autorewrite with RC.
@@ -55,26 +235,32 @@ Proof.
     replace emptyContext with (@empty Kind, mupd (msyn1 rho) empty).
     - eapply msubst_preserves_typing_1; eauto.
       eapply msubstA_preserves_typing_1; eauto.
-      destruct IH_LR.
-      eapply T_LamAbs; eauto.
+      eapply T_Let; eauto.
+      + eapply LR_la_bnr__oks in IH_LR__bs. 
+        apply IH_LR__bs.
+      + eapply IH_LR__t.
     - rewrite mupd_empty; eauto.
   }
   split. {
     replace emptyContext with (@empty Kind, mupd (msyn2 rho) empty).
-    - eapply msubst_preserves_typing_2; eauto.
+    - eapply LR_la_bnr__oks in IH_LR__bs as H.
+      eapply msubst_preserves_typing_2; eauto.
       eapply msubstA_preserves_typing_2; eauto.
-      destruct IH_LR. destruct H0.
-      eapply T_LamAbs; eauto.
+      eapply T_Let; eauto.
+      + apply H.
+      + destruct H. destruct H0. 
+        rewrite <- H1.
+        Fail rewrite <- Hbinds. (* why?? *)
+        unfold LR_logically_approximate in IH_LR__t.
+        apply skip.
     - rewrite mupd_empty; eauto.
   }
 
   intros j Hlt__j e_f Hev__e_f.
   inversion Hev__e_f. subst.
-  exists (LamAbs x (msubstT (msyn2 rho) T1) eb'_s).
-  exists 0.
-  split. {
-    eapply eval_value. apply V_LamAbs.
-  }
-  intros.
+  inversion H3. subst.
+  - unfold LR_logically_approximate in IH_LR__t.
+    destruct IH_LR__t as [_ [_ IH_LR__t]].
+    inversion Hbinds. subst. 
   *)
 Admitted.
