src/Language/PlutusIR/Semantics/SemanticEquivalence/CompatibilityLemmas/TermBind.v
@@ -1,0 +1,34 @@
+Require Import PlutusCert.Language.PlutusIR.
+Import NamedTerm.
+Require Import PlutusCert.Language.PlutusIR.Semantics.Dynamic.
+Require Import PlutusCert.Language.PlutusIR.Semantics.Static.
+Require Import PlutusCert.Language.PlutusIR.Semantics.SemanticEquivalence.LogicalRelation.RelationalModel.
+
+Lemma compatibility_TermBind : forall Delta Gamma stricty x T t t',
+    Delta |-* T : Kind_Base ->
+    LR_logically_approximate Delta Gamma t t' T ->
+    LR_logically_approximate_binding Delta Gamma (TermBind stricty (VarDecl x T) t) (TermBind stricty (VarDecl x T) t').
+Proof.
+  intros Delta Gamma stricty X T t t' Hkind__T IH_LR.
+  unfold LR_logically_approximate_binding.
+
+  split. {
+    eapply W_Term.
+    - apply Hkind__T. 
+    - apply IH_LR.
+  }
+  
+  split. {
+    eapply W_Term.
+    - apply Hkind__T.
+    - apply IH_LR.
+  }
+
+  intros k rho env env' ct ck HeqDelta HeqGamma [H_RD H_RG].
+  subst.
+
+  intros b_msa b'_msa b_ms b'_ms.
+  intros HmsA__b_msa HmsA__b'_msa Hms__b_s Hms__b'_s.
+
+  autorewrite with RB.
+Admitted.
