src/Language/PlutusIR/Semantics/SemanticEquivalence/CompatibilityLemmas/TypeBind.v
@@ -1,0 +1,24 @@
+Require Import PlutusCert.Language.PlutusIR.
+Import NamedTerm.
+Require Import PlutusCert.Language.PlutusIR.Semantics.Dynamic.
+Require Import PlutusCert.Language.PlutusIR.Semantics.Static.
+Require Import PlutusCert.Language.PlutusIR.Semantics.SemanticEquivalence.LogicalRelation.RelationalModel.
+
+Lemma compatibility_TypeBind : forall Delta Gamma X K T,
+    Delta |-* T : K ->
+    LR_logically_approximate_binding Delta Gamma (TypeBind (TyVarDecl X K) T) (TypeBind (TyVarDecl X K) T).
+Proof.
+  intros Delta Gamma X K T Hkind__T.
+  unfold LR_logically_approximate_binding.
+
+  split; eauto with typing.
+  split; eauto with typing.
+
+  intros k rho env env' ct ck HeqDelta HeqGamma [H_RD H_RG].
+  subst.
+
+  intros b_msa b'_msa b_ms b'_ms.
+  intros HmsA__b_msa HmsA__b'_msa Hms__b_s Hms__b'_s.
+
+  autorewrite with RB.
+Admitted.
